proof/invariants/MapMMUPage.v
@@ -30,7 +30,6 @@
 (*  The fact that you are presently reading this means that you have had       *)
 (*  knowledge of the CeCILL license and that you accept its terms.             *)
 (*******************************************************************************)
-
 (** * Summary 
     This file contains the invariant of [createPartition]. 
     We prove that this PIP service preserves the isolation property *)
