proof/invariants/UpdatePDFlagTrue.v
@@ -30,7 +30,6 @@
 (*  The fact that you are presently reading this means that you have had       *)
 (*  knowledge of the CeCILL license and that you accept its terms.             *)
 (*******************************************************************************)
-
 Require Import Model.ADT Model.Hardware Core.Services Isolation
 Consistency Invariants WeakestPreconditions Model.Lib StateLib
 Model.MAL UpdateShadow1Structure InternalLemmas DependentTypeLemmas Lib
