proof/invariants/mapInChild.v
@@ -1,0 +1,336 @@
+(*******************************************************************************)
+(*  © Université Lille 1, The Pip Development Team (2015-2017)                 *)
+(*                                                                             *)
+(*  This software is a computer program whose purpose is to run a minimal,     *)
+(*  hypervisor relying on proven properties such as memory isolation.          *)
+(*                                                                             *)
+(*  This software is governed by the CeCILL license under French law and       *)
+(*  abiding by the rules of distribution of free software.  You can  use,      *)
+(*  modify and/ or redistribute the software under the terms of the CeCILL     *)
+(*  license as circulated by CEA, CNRS and INRIA at the following URL          *)
+(*  "http://www.cecill.info".                                                  *)
+(*                                                                             *)
+(*  As a counterpart to the access to the source code and  rights to copy,     *)
+(*  modify and redistribute granted by the license, users are provided only    *)
+(*  with a limited warranty  and the software's author,  the holder of the     *)
+(*  economic rights,  and the successive licensors  have only  limited         *)
+(*  liability.                                                                 *)
+(*                                                                             *)
+(*  In this respect, the user's attention is drawn to the risks associated     *)
+(*  with loading,  using,  modifying and/or developing or reproducing the      *)
+(*  software by the user in light of its specific status of free software,     *)
+(*  that may mean  that it is complicated to manipulate,  and  that  also      *)
+(*  therefore means  that it is reserved for developers  and  experienced      *)
+(*  professionals having in-depth computer knowledge. Users are therefore      *)
+(*  encouraged to load and test the software's suitability as regards their    *)
+(*  requirements in conditions enabling the security of their systems and/or   *)
+(*  data to be ensured and,  more generally, to use and operate it in the      *)
+(*  same conditions as regards security.                                       *)
+(*                                                                             *)
+(*  The fact that you are presently reading this means that you have had       *)
+(*  knowledge of the CeCILL license and that you accept its terms.             *)
+(*******************************************************************************)
+
+Require Import Model.ADT Model.Hardware Core.Services Isolation 
+Consistency WeakestPreconditions Invariants StateLib Model.Lib
+ Model.MAL GetTableAddr InternalLemmas DependentTypeLemmas.
+Require Import Omega Bool List.
+
+(** * Summary 
+    This file contains the invariant of [addVaddr]. 
+    We prove that this PIP service preserves the isolation property *)
+
+Lemma mappedInChild (vaChild : vaddr) :
+{{fun s => partitionsIsolation s   /\ kernelDataIsolation s /\ verticalSharing s /\ consistency s }} 
+mappedInChild vaChild 
+{{fun _ s  => partitionsIsolation s   /\ kernelDataIsolation s /\ verticalSharing s /\ consistency s }}.
+Proof.
+unfold mappedInChild.
+(** getCurPartition **)
+eapply WP.bindRev.
+eapply WP.weaken. 
+eapply Invariants.getCurPartition .
+cbn. 
+intros. 
+pattern s in H. 
+eexact H.
+intro currentPart.
+(** getNbLevel **)
+eapply WP.bindRev.
+eapply weaken.
+eapply Invariants.getNbLevel.
+simpl. intros.
+pattern s in H.
+eexact H.
+intros level.
+simpl.
+(** getPd **)  
+eapply WP.bindRev. 
+{ eapply WP.weaken. 
+  eapply Invariants.getPd.
+  simpl.
+  intros.
+  split.
+  (* try repeat rewrite and_assoc in H. *)
+  pattern s in H. eapply H.
+  unfold consistency in *.
+  unfold partitionDescriptorEntry in *.
+  unfold currentPartitionInPartitionsList in *.
+  intuition          subst. trivial. 
+  }
+intro currentPD. simpl. 
+(** getTableAddr **)
+      eapply WP.bindRev.
+      eapply WP.weaken. 
+      apply getTableAddr.
+      simpl.
+      intros s H.
+      try repeat rewrite and_assoc in H.
+      split.
+      pattern s in H. 
+      eapply H. subst.
+      split. 
+      intuition.
+      split. 
+      instantiate (1:= currentPart). 
+      intuition. 
+      subst.
+      unfold consistency in *. 
+      unfold  currentPartitionInPartitionsList in *. 
+      intuition.
+      instantiate (1:= PDidx).
+      split. intuition.
+      assert(consistency s /\
+              Some level = StateLib.getNbLevel /\ 
+              currentPart = currentPartition s /\ 
+              nextEntryIsPP currentPart PDidx currentPD s) as (Hcons & Hlevel & Hcp & Hrootpd)
+      by intuition.
+      clear H. 
+      exists currentPD.
+      split. assumption.
+      split.
+      unfold consistency in *.
+      assert(partitionDescriptorEntry s /\ currentPartitionInPartitionsList s) as (Hpd &Hpr)
+      by intuition. clear Hcons. 
+
+      unfold partitionDescriptorEntry in Hpd.
+      assert (PDidx = PDidx \/ PDidx = sh1idx \/ PDidx = sh2idx\/PDidx = sh3idx\/ PDidx = PPRidx \/ PDidx = PRidx ) as Htmp
+          by auto.
+      subst.
+      generalize (Hpd  (currentPartition s)  Hpr); clear Hpd; intros Hpd.     
+       generalize (Hpd PDidx Htmp); clear Hpd; intros Hpd.
+      destruct Hpd as (Hidxpd & _& Hentry).
+      destruct Hentry as (page1 & Hpd & Hnotnull).
+      subst.
+      unfold nextEntryIsPP in *; destruct (StateLib.Index.succ PDidx);
+       [destruct (lookup (currentPartition s) i (memory s) beqPage beqIndex)
+       as [v |]; [ destruct v as [ p |v|p|v|ii] ; [ now contradict Hrootpd | now contradict Hrootpd | 
+       subst ; assumption| now contradict Hrootpd| now contradict Hrootpd ]  |now contradict Hrootpd] | now contradict Hrootpd].
+
+      subst. left. split;intuition.
+     intro ptvaChildFromPD. simpl.
+
+ (** simplify the new precondition **)     
+      eapply WP.weaken.
+      intros.
+      Focus 2.
+      intros.
+      destruct H as (H0 & H1).
+      assert(( getTableAddrRoot' ptvaChildFromPD PDidx currentPart vaChild s /\  ptvaChildFromPD = defaultPage) \/
+     (forall idx : index,
+      StateLib.getIndexOfAddr vaChild fstLevel = idx ->
+      isPE ptvaChildFromPD idx s/\
+     getTableAddrRoot ptvaChildFromPD PDidx currentPart vaChild s)).
+      {
+      destruct H1 as [H1 |(Hnew & Hi & H1)].
+      + left. trivial. 
+      + right. intros idx Hidx.
+      
+        generalize (H1 idx Hidx);clear H1;intros H1.
+        destruct H1 as [(_& Hfalse) | [(_&Hfalse) |(Hpe &Htrue)]].
+        - contradict Hfalse. apply idxPDidxSh1notEq.
+       - contradict Hfalse. apply idxPDidxSh2notEq.
+      -split;
+       assumption. }
+       
+       assert (HP := conj H0 H).
+       pattern s in HP.
+       eapply HP.   
+(** comparePageToNull **) 
+      eapply WP.bindRev.
+      eapply Invariants.comparePageToNull.
+      intro ptvachildIsnull. simpl.
+      case_eq ptvachildIsnull.
+      { intros. eapply WP.weaken.  eapply WP.ret . simpl. intros. intuition. }
+      intros HisNullpd. subst.
+(** StateLib.getIndexOfAddr    *)             
+      eapply WP.bindRev.
+      eapply WP.weaken.
+      eapply Invariants.getIndexOfAddr.
+      { simpl. intros. 
+        destruct H as ((H & [(Hptchild & Hi)| Hptchild]) & Hptchildnotnull).
+        + subst. contradict Hptchildnotnull. intro Hnull.  apply beq_nat_false in Hnull. intuition.
+        + subst.
+          assert (HP := conj (conj H Hptchild) Hptchildnotnull).
+(*           try repeat rewrite and_assoc in H. *)
+          pattern s in HP.
+          eapply HP.  }
+       intro idxSh1. simpl.
+(**readPresent **)
+       eapply WP.bindRev.
+       { eapply WP.weaken.
+         eapply Invariants.readPresent. simpl.
+         intros.
+         split. 
+(*          try repeat rewrite and_assoc in H. *)
+         pattern s in H.
+         eapply H. 
+         subst.
+         destruct H as (H & Hidx).
+         assert (forall idx : index,
+         StateLib.getIndexOfAddr vaChild fstLevel = idx -> 
+         isPE ptvaChildFromPD idx s /\
+     getTableAddrRoot ptvaChildFromPD PDidx currentPart vaChild s).  
+         { intuition. }
+         
+         apply H0 in Hidx. destruct Hidx; assumption.
+       }
+       intro present. simpl.
+(**readAccessible **)
+       eapply WP.bindRev.
+       { eapply WP.weaken.
+         eapply Invariants.readAccessible. simpl.
+         intros.
+         split.
+         
+(*          try repeat rewrite and_assoc in H. *)
+         pattern s in H.
+         eapply H. 
+         subst.
+         apply entryPresentFlagIsPE with present;intuition. }
+       intros accessible. simpl.   
+case_eq(present && accessible);intros Hand.
+(** getFstShadow **)
+eapply bindRev.
+eapply WP.weaken. 
+eapply Invariants.getFstShadow. cbn.
+intros s H.
+split.
+pattern s in H.
+eexact H.
+unfold consistency in *.
+unfold partitionDescriptorEntry in *.
+intuition.
+simpl.
+intros currentShadow.
+(** getTableAddr : to check if the virtual address is available to map a new page  **)
+eapply WP.bindRev.
+eapply WP.weaken. 
+apply getTableAddr.
+simpl.
+intros s H.  
+split. 
+pattern s in H. 
+eexact H. subst.
+split. 
+intuition.
+
+split. 
+instantiate (1:= currentPart );trivial.
+{ unfold consistency in *. 
+unfold currentPartitionInPartitionsList in *.
+intuition. subst. trivial. }
+instantiate (1:= sh1idx).
+split. intuition.
+assert(Hcons : consistency s) by intuition.
+assert(Hlevel : Some level = StateLib.getNbLevel) by intuition. 
+assert(Hcp : currentPart = currentPartition s) by intuition.
+exists currentShadow.
+split. intuition.
+split. 
+apply sh1PartNotNull with currentPart s.
+{ unfold consistency in *. 
+unfold currentPartitionInPartitionsList in *.
+intuition. subst. trivial. } 
+intuition.
+unfold consistency in *.
+intuition.
+left.
+split;trivial.
+intros ptVaChildFromSh1.
+(** simplify the new precondition **)     
+eapply WP.weaken.
+intros.
+Focus 2.
+intros.
+destruct H as (H0 & H1).
+assert ( (getTableAddrRoot' ptVaChildFromSh1 sh1idx currentPart vaChild s /\ 
+ptVaChildFromSh1 = defaultPage) \/
+(forall idx : index,
+StateLib.getIndexOfAddr vaChild fstLevel = idx ->
+isVE ptVaChildFromSh1 idx s /\ getTableAddrRoot ptVaChildFromSh1 sh1idx currentPart vaChild s  )).
+{ destruct H1 as [H1 |(Hi & Hi1 & H1)].
+  + left. trivial. 
+  + right. intros idx Hidx.
+    generalize (H1 idx Hidx);clear H1;intros H1.
+    destruct H1 as [(Hpe &Htrue) |[ (Hpe& Hfalse) | (Hpe&Hfalse) ]].
+    -  split; assumption.
+    - contradict Hfalse.
+       unfold not;intros Hfalse;symmetry in Hfalse; contradict Hfalse.
+      apply idxSh2idxSh1notEq.
+    - contradict Hfalse. 
+      unfold not;intros Hfalse;symmetry in Hfalse; contradict Hfalse.
+      apply idxPDidxSh1notEq. }
+assert (HP := conj H0 H).
+pattern s in HP.
+exact HP.
+(** comparePageToNull **) 
+eapply WP.bindRev.
+eapply Invariants.comparePageToNull.
+intro isNull. simpl.
+case_eq isNull.
+{ intros. eapply WP.weaken.
+  eapply WP.ret . simpl.
+  intros. intuition. }
+intros HisNull. subst.
+(** StateLib.getIndexOfAddr **)                
+eapply WP.bindRev.
+eapply WP.weaken.
+eapply Invariants.getIndexOfAddr.
+{ simpl. intros.
+  destruct H as ((Ha1 & Ha3) & Ha4).
+  assert (Hnewget :  isVE ptVaChildFromSh1
+  (StateLib.getIndexOfAddr vaChild fstLevel) s /\
+       getTableAddrRoot ptVaChildFromSh1 sh1idx currentPart vaChild s /\ 
+       (defaultPage =? ptVaChildFromSh1) = false).
+  { destruct Ha3 as [(Ha3 & Hfalse) | Ha3].
+    + subst.
+      apply beq_nat_false in Ha4.
+      now contradict Ha4.
+    + destruct Ha3 with (StateLib.getIndexOfAddr vaChild fstLevel);trivial.
+      intuition. }
+   subst.
+  assert (HP := conj Ha1 Hnewget).
+  pattern s in HP.
+  eexact HP. }
+intro idxvaChild.
+simpl.
+(** readVirEntry **)
+eapply WP.weaken.
+eapply WP.readVirEntry. simpl.
+intros.
+destruct H as (H & Hentry).
+assert(Hx : isVE ptVaChildFromSh1 (StateLib.getIndexOfAddr vaChild fstLevel) s ) by intuition.
+unfold isVE in Hx.
+subst.
+destruct (lookup ptVaChildFromSh1 (StateLib.getIndexOfAddr vaChild fstLevel)
+         (memory s) beqPage beqIndex);
+         try now contradict Hx.
+destruct v ; try now contradict Hx.
+exists v.
+split;intuition.
+(** ret **)
+eapply weaken.
+eapply WP.ret . simpl.
+  intros. intuition.
+Qed.
