src/model/ADT.v
@@ -58,11 +58,8 @@ Axiom nbPageNotZero: nbPage > 0.
 
 Axiom tableSizeIsEven : Nat.Even tableSize.
 (* END NOT SIMULATION *)
-Definition tableSizeLowerBound := 14.
-
+Definition tableSizeLowerBound := 14.  
 Axiom tableSizeBigEnough : tableSize > tableSizeLowerBound. (* to be fixed on count **) 
-
-Definition preIndex := nat.
 Record index := {
   i :> nat ;
   Hi : i < tableSize }.
@@ -73,12 +70,10 @@ Record page := {
 
 Definition paddr := (page * index)%type.
 
-Definition preVaddr := (list nat).
 Record vaddr := {
   va :> list index ;
   Hva : length va = nbLevel + 1}.
 
-Definition preLevel := nat.
 Record level := {
   l :> nat ;
   Hl : l < nbLevel }.
@@ -88,8 +83,6 @@ Record count := {
   Hnb : c <= (3*nbLevel) + 1  ;
  }.
 
-
-Parameter preIndex_d : preIndex.
 Parameter index_d : index.
 Parameter page_d : page.
 Parameter level_d : level.
